x86/SSAsm.v
@@ -3,7 +3,7 @@ Require Import AST Integers Floats Values Memory Events Globalenvs Smallstep.
 Require Import Locations Conventions.
 Require Import Asm.
 
-Definition stkblock := Stack Mem.pid None nil 1.
+Definition stkblock := Stack Mem.tid None nil 1.
 
 Section SSASM.
 
